temp stuff

src/Std/Data/TreeMap/Basic.lean
@@ -71,6 +71,13 @@ instance : EmptyCollection (TreeMap α β cmp) where
 
 instance : Inhabited (TreeMap α β cmp) := ⟨∅⟩
 
+@[inherit_doc DTreeMap.Equiv]
+structure Equiv (m₁ m₂ : TreeMap α β cmp) where
+  /-- Internal implementation detail of the hash map -/
+  inner : m₁.1.Equiv m₂.1
+
+@[inherit_doc] scoped infix:50 " ~m " => Equiv
+
 @[simp]
 theorem empty_eq_emptyc : (empty : TreeMap α β cmp) = ∅ :=
   rfl
